new host actions call_wasm and modify_table have been added and their wp_rules proved

theories/iris/iris_host.v
@@ -39,10 +39,8 @@ Inductive host_action : Type :=
 | HA_nothing : host_action
 | HA_print : host_action
 | HA_instantiate : inst_decl -> host_action
-(*  (* Some ideas for future additional actions : *)
 | HA_call_wasm : host_action
 | HA_modify_table : host_action
-*)
 .
 
 
@@ -100,17 +98,28 @@ Fixpoint insert_exports (vis: vi_store) (iexps: list vi) (exps: list module_expo
 Definition empty_instance := Build_instance [::] [::] [::] [::] [::].
 Definition empty_frame := Build_frame [::] empty_instance.
 
-(* Dummy *)
-(* Parameter hs: host_state host_instance. *)
+Print store_record. 
+Definition stab_update s i idx newval :=
+  match List.nth_error (s_tables s) i with 
+  | None => None
+  | Some stab_i =>
+      if length (table_data stab_i) <? idx then None
+      else
+        Some {| s_funcs := s_funcs s ;
+               s_mems := s_mems s ;
+               s_globals := s_globals s ;
+               s_tables := update_list_at (s_tables s) i
+                                          {| table_data := update_list_at (table_data stab_i) idx (Some newval) ;
+                                            table_max_opt := table_max_opt stab_i |}
+             |} 
+  end.
 
-(* Note that instantiation takes imports as module_export_desc but gives exports as module_export (i.e. with a name). *)
 
-(*
-Inductive local_label_holed : Type :=
-| LL_base : list value -> list administrative_instruction -> local_label_holed
-| LL_local : list value -> nat -> frame -> local_label_holed -> list administrative_instruction -> local_label_holed
-| LL_label : list value -> nat -> list administrative_instruction -> local_label_holed -> list administrative_instruction -> local_label_holed.
-*)
+Definition update_table s f idx newval :=
+   match f.(f_inst).(inst_tab) with
+  | nil => None
+  | ta :: q => stab_update s ta idx newval
+  end.
 
 
 
@@ -137,13 +146,13 @@ Inductive host_reduce: store_record -> vi_store -> list module -> list inst_decl
   forall (s:store_record) vis ms idecs (s':store_record) (tf:function_type)
     (h:hostfuncidx) (hi:nat) f
     (vcs:seq.seq value) fs
-    (res : seq.seq administrative_instruction) (LI : seq.seq administrative_instruction) LI' lh f0,
+    (res : seq.seq administrative_instruction) (LI : seq.seq administrative_instruction) LI' lh f0 f1,
     h = Mk_hostfuncidx hi ->
     fs !! hi = Some f ->
-    execute_action f s vcs s' res ->
+    execute_action f s f0 vcs s' f1 res ->
     llfill lh [AI_call_host tf h vcs] = LI ->
     llfill lh res = LI' ->
-    host_reduce s vis ms idecs fs f0 LI s' vis ms idecs fs f0 LI'
+    host_reduce s vis ms idecs fs f0 LI s' vis ms idecs fs f1 LI'
 | HR_call_host_instantiate :
   forall s vis ms idecs h hi f fs LI LI' lh f0,
     h = Mk_hostfuncidx hi ->
@@ -151,37 +160,20 @@ Inductive host_reduce: store_record -> vi_store -> list module -> list inst_decl
     llfill lh [AI_call_host (Tf [] []) h []] = LI ->
     llfill lh [] = LI' ->
     host_reduce s vis ms idecs fs f0 LI s vis ms (f :: idecs) fs f0 LI' 
-(* | HR_call_host_action :
-  forall s vis ms idecs s' tf h hi f vcs fs res f0,
-    h = Mk_hostfuncidx hi ->
-    fs !! hi = Some f ->
-    execute_action f s vcs s' res ->
-    host_reduce s vis ms idecs fs f0 [AI_call_host tf h vcs] s' vis ms idecs fs f0 res
-| HR_call_host_instantiate :
-  forall s vis ms idecs h hi f fs f0,
-    h = Mk_hostfuncidx hi ->
-    fs !! hi = Some (HA_instantiate f) ->
-    host_reduce s vis ms idecs fs f0 [AI_call_host (Tf [] []) h []] s vis ms (f :: idecs) fs f0 []
-| HR_local :
-  forall s vis ms idecs fs f0 n f es s' vis' ms' idecs' fs' f' es',
-    const_list es = false ->
-    host_reduce s vis ms idecs fs f es s' vis' ms' idecs' fs' f' es' ->
-    host_reduce s vis ms idecs fs f0 [AI_local n f es] s' vis' ms' idecs' fs' f0 [AI_local n f' es']
-| HR_label :
-  forall k lh es LI es' LI' s vis ms idecs fs f s' vis' ms' idecs' fs' f',
-    const_list es = false ->
-    lfilled k lh es LI ->
-    lfilled k lh es' LI' ->
-    host_reduce s vis ms idecs fs f es s' vis' ms' idecs' fs' f' es' ->
-    host_reduce s vis ms idecs fs f LI s' vis' ms' idecs' fs' f' LI'*) 
 | HR_wasm_step: forall s vis ms idecs s' es es' f1 f2 fs,
     opsem.reduce s f1 es s' f2 es' ->
     host_reduce s vis ms idecs fs f1 es s' vis ms idecs fs f2 es'
 
                 
-with execute_action : host_action -> store_record -> list value -> store_record -> list administrative_instruction -> Prop :=
-| execute_nothing : forall s, execute_action HA_nothing s [] s []
-| execute_print : forall s v, execute_action HA_print s [v] s []
+with execute_action : host_action -> store_record -> frame -> list value -> store_record -> frame -> list administrative_instruction -> Prop :=
+| execute_nothing : forall s f, execute_action HA_nothing s f [] s f []
+| execute_print : forall s f v, execute_action HA_print s f [v] s f []
+| execute_call_wasm : forall s f i, execute_action HA_call_wasm s f [VAL_int32 i] s f [AI_basic (BI_call (Wasm_int.nat_of_uint i32m i))]
+| execute_modify_table : forall s f tab_idx func_idx s' a,
+    List.nth_error f.(f_inst).(inst_funcs) (Wasm_int.nat_of_uint i32m func_idx) = Some a ->
+    update_table s f (Wasm_int.nat_of_uint i32m tab_idx) a = Some s' ->
+    execute_action HA_modify_table s f [VAL_int32 tab_idx ; VAL_int32 func_idx]
+                   s' f []
 .
 
 
@@ -355,12 +347,15 @@ Proof.
 Qed.
 *)
 
-Lemma execute_action_det f s vcs s1 res1 s2 res2 :
-  execute_action f s vcs s1 res1 -> execute_action f s vcs s2 res2 ->
-  s1 = s2 /\ res1 = res2.
+Lemma execute_action_det f s vcs s1 f0 f1 res1 s2 f2 res2 :
+  execute_action f s f0 vcs s1 f1 res1 -> execute_action f s f0 vcs s2 f2 res2 ->
+  s1 = s2 /\ res1 = res2 /\ f1 = f2.
 Proof.
   intros Hea1 Hea2.
   inversion Hea1 ; inversion Hea2 ; subst => //.
+  inversion H9 => //.
+  inversion H13 ; subst. rewrite H in H8. inversion H8 ; subst.
+  rewrite H0 in H9. by inversion H9. 
 Qed.
 
 
@@ -383,7 +378,7 @@ Proof.
       apply llfill_unique in H2 as [[H ->] | [? | [? | [ (?&?&?&[?|?]) | (?&?&?&[?|?])]]]] => //=.
       inversion H ; subst.
       rewrite H0 in H5. inversion H5 ; subst.
-      destruct (execute_action_det _ _ _ _ _ _ _ H1 H6) as [-> ->] => //. 
+      destruct (execute_action_det _ _ _ _ _ _ _ _ _ _ H1 H6) as (-> & -> & ->) => //. 
     + simplify_eq. rewrite - H6 in H2. 
       apply llfill_unique in H2 as [[H ->] | [? | [? | [ (?&?&?&[?|?]) | (?&?&?&[?|?])]]]] => //=.
       inversion H ; subst.
@@ -603,13 +598,13 @@ Section host_lifting.
 Context `{!wasmG Σ, !hvisG Σ, !hmsG Σ, !hasG Σ}.
 
 
-Lemma wp_call_host_action s E hes tf h hi f vcs (Φ : host_val -> iProp Σ) res llh LI LI' :
+Lemma wp_call_host_action_no_state_change s E hes tf h hi f vcs (Φ : host_val -> iProp Σ) res llh LI LI' :
   h = Mk_hostfuncidx hi ->
   llfill llh [AI_call_host tf h vcs] = LI ->
   llfill llh res = LI' ->
-  (forall s0, execute_action f s0 vcs s0 res) -> (* so far no executable action requires knowledge of the store_record so this hypothesis is enough for all usage. Later, we may need stronger versions of this lemma for stronger host_actions, with extra iris-hypotheses about the exact form of the store_record *)
+  (forall s0 f0, execute_action f s0 f0 vcs s0 f0 res) -> 
   N.of_nat hi ↦[ha] f ∗ WP ((hes, LI') : host_expr) @ s ; E {{ v, Φ v  }}
-  ⊢ WP ((hes, LI) : host_expr) @ s ; E {{ v, Φ v }}.
+  ⊢ WP ((hes, LI) : host_expr) @ s ; E {{ v, Φ v ∗ N.of_nat hi ↦[ha] f }}.
 Proof.
   iIntros (Hh HLI HLI' Hexec) "(Hhi & Hwp)".
   iApply lifting.wp_lift_step => //=.
@@ -639,7 +634,7 @@ Proof.
     eapply call_host_reduce_det in HStep ; last first.
     eapply HR_call_host_action => //=.
     exact HLI. inversion HStep ; subst.
-    iFrame. done.  
+    iFrame. iFrame. done.  
 Qed.
   
 
@@ -649,7 +644,7 @@ Lemma wp_call_host_instantiate s E hes h hi f (Φ : host_val -> iProp Σ) llh LI
   llfill llh [AI_call_host (Tf [] []) h []] = LI ->
   llfill llh [] = LI' ->
   N.of_nat hi ↦[ha] (HA_instantiate f) ∗  WP ((f :: hes, LI') : host_expr) @ s ; E {{ v, Φ v }}
-  ⊢ WP ((hes, LI) : host_expr) @ s ; E {{ v, Φ v }}.
+  ⊢ WP ((hes, LI) : host_expr) @ s ; E {{ v, Φ v ∗ N.of_nat hi ↦[ha] (HA_instantiate f) }}.
 Proof.
   iIntros (Hh HLI HLI') "(Hhi & Hwp)".
   iApply lifting.wp_lift_step => //=.
@@ -679,7 +674,118 @@ Proof.
     eapply call_host_reduce_det in HStep ; last first.
     eapply HR_call_host_instantiate => //=.
     exact HLI. inversion HStep ; subst.
-    iFrame. done.  
+    iFrame. iFrame. done.  
+Qed.
+
+Lemma nth_error_none_fmap {A B} (l : seq.seq A) n (f : A -> B) :
+  nth_error l n = None -> nth_error (f <$> l) n = None.
+Proof.
+  generalize dependent l ; induction n ; intros.
+  destruct l => //.
+  destruct l => //=.
+  apply IHn => //.
+Qed.
+
+Lemma fmap_update_list_at {A B} l i x (f : A -> B) :
+  f <$> update_list_at l i x = update_list_at (f <$> l) i (f x).
+Proof.
+  unfold update_list_at.
+  rewrite fmap_app => /=.
+  rewrite take_fmap. rewrite - fmap_drop. done.
+Qed. 
+
+
+Lemma wp_call_host_modify_table s E h hi tab_idx func_idx LI LI' llh f0 n func_idx0 hes a Φ :
+  h = Mk_hostfuncidx hi ->
+  llfill llh [AI_call_host (Tf [T_i32 ; T_i32] []) h [VAL_int32 tab_idx ; VAL_int32 func_idx]] = LI ->
+  llfill llh [] = LI' ->
+  f0.(f_inst).(inst_funcs) !! (Wasm_int.nat_of_uint i32m func_idx) = Some a -> 
+  f0.(f_inst).(inst_tab) !! 0 = Some n ->
+  ↪[frame] f0 ∗
+   N.of_nat hi ↦[ha] HA_modify_table ∗
+   N.of_nat n ↦[wt][ Wasm_int.N_of_uint i32m tab_idx ] func_idx0 ∗
+   WP ((hes, LI') : host_expr) @ s ; E {{ Φ }}
+   ⊢ WP ((hes, LI) : host_expr) @ s ; E {{ v, Φ v ∗
+                                                ↪[frame] f0 ∗
+                                                N.of_nat hi ↦[ha] HA_modify_table ∗
+                                                N.of_nat n ↦[wt][ Wasm_int.N_of_uint i32m tab_idx ] Some a }}.
+Proof.
+  iIntros (Hh HLI HLI' Ha Hn) "(Hf & Hhi & Hwt & Hwp)".
+  iApply lifting.wp_lift_step => //=.
+  - destruct hes => //. subst.
+    fold (iris.of_val (callHostV (Tf [T_i32 ; T_i32] []) (Mk_hostfuncidx hi) [VAL_int32 tab_idx ; VAL_int32 func_idx ] llh)).
+    rewrite iris.to_of_val => //. 
+  - iIntros (σ ns κ κs nt) "Hσ".
+    destruct σ as [[[[ws vi] ms] has] f1].
+    iDestruct "Hσ" as "(Hfunc & Htab & ? & ? & ? & ? & Hha & Hf1 & ? & Htabsize & ? & ?)".
+    iDestruct (ghost_map_lookup with "Hha Hhi") as "%Hha".
+    rewrite gmap_of_list_lookup Nat2N.id in Hha.
+    rewrite - nth_error_lookup in Ha.
+    iDestruct (ghost_map_lookup with "Hf1 Hf") as "%Hf0".
+    rewrite lookup_insert in Hf0. inversion Hf0 ; subst ; clear Hf0.
+    destruct (inst_tab (f_inst f0)) eqn:Hf => //.
+    simpl in Hn ; inversion Hn ; subst ; clear Hn.
+    iDestruct (gen_heap_valid with "Htab Hwt") as "%H".
+    simplify_lookup.
+    rewrite - nth_error_lookup in Heq.
+    destruct (nth_error (s_tables ws) n) eqn:Htables.
+    2:{ apply (nth_error_none_fmap _ _ table_to_list) in Htables.
+        rewrite Htables in Heq. done. }
+    rewrite (map_nth_error table_to_list _ _ Htables) in Heq.
+    inversion Heq ; subst ; clear Heq.
+    unfold table_to_list in H.
+    specialize (lookup_lt_Some _ _ _ H) as Hlt.
+    replace (N.to_nat (Z.to_N (Wasm_int.Int32.unsigned tab_idx))) with
+      (Wasm_int.nat_of_uint i32m tab_idx) in Hlt ; last by rewrite Z_N_nat.
+    iApply fupd_mask_intro ; first by solve_ndisj.
+    iIntros "Hfupd".
+    iSplit.
+  - iPureIntro.
+    destruct s => //=.
+    unfold language.reducible, language.prim_step => /=.
+    eexists [], (_,_), (_,_,_,_,_), [].
+    repeat split => //=.
+    eapply HR_call_host_action => //.
+    eapply execute_modify_table => //.
+    unfold update_table. 
+    rewrite Hf. unfold stab_update.
+    rewrite Htables. 
+    destruct (length (table_data t) <? _) eqn:Habs'.
+    apply ltb_lt in Habs'. lia.
+    done.
+  - iIntros "!>" (es σ2 efs HStep).
+    destruct σ2 as [[[[s2 vi2] ms2] has2] f2].
+    destruct es as [hes2 es2].
+    destruct HStep as [HStep [-> ->]].
+    eapply call_host_reduce_det in HStep ; last first.
+    eapply HR_call_host_action => //=.
+    eapply execute_modify_table => //.
+    2: done.
+    unfold update_table. rewrite Hf. unfold stab_update. rewrite Htables.
+    unfold table_to_list in H. destruct (_ <? _) eqn:Habs.
+    apply ltb_lt in Habs. lia. done. 
+    inversion HStep ; subst. simpl.
+    iMod (gen_heap_update with "Htab Hwt") as "[Htab Hwt]".
+    iMod "Hfupd".
+    instantiate (1:= Some a). 
+    iFrame. repeat rewrite fmap_update_list_at => /=.
+    rewrite (update_trivial (table_max_opt <$> _)).
+    rewrite (update_trivial (tab_size <$> _)). iFrame.
+    erewrite gmap_of_table_insert.
+    rewrite Nat2N.id. 
+    repeat rewrite update_list_at_insert.
+    instantiate (1 := t).
+    rewrite Z_N_nat. done.
+    simpl in Hlt. done.
+    rewrite nth_error_lookup in Htables ; apply lookup_lt_Some in Htables. done.
+    rewrite Nat2N.id. by rewrite - nth_error_lookup.
+    rewrite Z_N_nat. done.
+    apply (map_nth_error tab_size) in Htables.
+    rewrite nth_error_lookup in Htables.
+    rewrite Htables. unfold tab_size => /=.
+    rewrite update_length => //.
+    apply (map_nth_error table_max_opt) in Htables.
+    rewrite nth_error_lookup in Htables. done. 
 Qed.
 
 
